Week 3 sheets

src/section03groups/sheet4.lean
@@ -33,6 +33,7 @@ notation G ` →** ` H := my_group_hom G H
 -- A group hom is a function, and so we set up a "coercion"
 -- so that a group hom can be regarded as a function (even
 -- though it's actually a pair consisting of a function and an axiom)
+-- instance : has_coe (G →** H) (G → H) := { coe := my_group_hom.to_fun }
 instance : has_coe_to_fun (G →** H) (λ _, G → H) :=
 { coe := my_group_hom.to_fun }
 
@@ -60,12 +61,18 @@ variable (f : G →** H)
 -- Now see if you can do these.
 @[simp] lemma map_one : f 1 = 1 :=
 begin
-  sorry
+  have : f 1 = f 1 := by simp,
+  nth_rewrite 0 ←mul_one (1 : G) at this,
+  rw map_mul at this,
+  exact mul_right_eq_self.mp this,
 end
 
 lemma map_inv (a : G) : f a⁻¹ = (f a)⁻¹ :=
 begin
-  sorry,
+  have := map_one f,
+  rw ←mul_inv_self a at this,
+  rw map_mul at this,
+  exact (inv_eq_of_mul_eq_one this).symm,
 end
 
 variable (G)
@@ -73,64 +80,101 @@ variable (G)
 /-- `id G` is the identity group homomorphism from `G` to `G`. -/
 def id : G →** G :=
 { to_fun := λ a, a,
-  map_mul' := begin sorry end } -- fill in the proof that the identity function is a group hom!
+  map_mul' := by simp } -- fill in the proof that the identity function is a group hom!
 
 variables {K : Type} [group K] {G}
 
 /-- `φ.comp ψ` is the composite of `φ` and `ψ`. -/
 def comp (φ : G →** H) (ψ : H →** K) : G →** K :=
 { to_fun := λ g, ψ (φ g),
-  map_mul' := begin sorry end -- fill in the proof that composite of two group homs is a group hom!
+  map_mul' := begin intros, rw map_mul, rw map_mul, end -- fill in the proof that composite of two group homs is a group hom!
 }
 
 -- The next three lemmas are pretty standard, but they are also in fact
 -- the axioms that show that groups form a category.
 lemma id_comp : (id G).comp f = f :=
 begin
-  sorry
+  ext,
+  refl,
 end
 
 lemma comp_id : f.comp (id H) = f :=
 begin
-  sorry
+  ext,
+  refl,
 end
 
 lemma comp_assoc {L : Type} [group L] (φ : G →** H) (ψ : H →** K) (ρ : K →** L) :
   (φ.comp ψ).comp ρ = φ.comp (ψ.comp ρ) :=
 begin
-  sorry,
+  ext,
+  refl,
 end
 
 /-- The kernel of a group homomorphism, as a subgroup of the source group. -/
 def ker (f : G →** H) : subgroup G :=
 { carrier := {g : G | f g = 1 },
-  one_mem' := begin sorry end,
-  mul_mem' := begin sorry end,
-  inv_mem' := begin sorry end,
+  one_mem' := begin exact map_one f end,
+  mul_mem' := begin intros a b ha hb, simp [map_mul, *] at *,  end,
+  inv_mem' := begin intros x hx, simp [map_inv, *] at *, end,
 }
 
 /-- The image of a group homomorphism, as a subgroup of the target group. -/
 def im (f : G →** H) : subgroup H :=
 { carrier := {h : H | ∃ g : G, f g = h },
-  one_mem' := begin sorry end,
-  mul_mem' := begin sorry end,
-  inv_mem' := begin sorry end,
+  one_mem' := begin use 1, simp, end,
+  mul_mem' :=
+  begin
+    intros a b ha hb,
+    cases ha with a' ha,
+    cases hb with b' hb,
+    use a' * b',
+    simp [map_mul, *],
+  end,
+  inv_mem' :=
+  begin
+    intros x hx,
+    cases hx with x' hx,
+    use x'⁻¹,
+    simp [map_inv, *],
+  end,
 }
 
 /-- The image of a subgroup under a group homomorphism, as a subgroup. -/
 def map (f : G →** H) (K : subgroup G) : subgroup H :=
 { carrier := {h : H | ∃ g : G, g ∈ K ∧ f g = h },
-  one_mem' := begin sorry end,
-  mul_mem' := begin sorry end,
-  inv_mem' := begin sorry end,
+  one_mem' := begin use 1, simp [map_one, K.one_mem], end,
+  mul_mem' :=
+  begin
+    intros a b ha hb,
+    cases ha with a' ha,
+    cases hb with b' hb,
+    use a' * b',
+    simp [map_mul, K.mul_mem, *],
+  end,
+  inv_mem' :=
+  begin
+    intros x hx,
+    cases hx with x' hx,
+    use x'⁻¹,
+    simp [map_inv, K.inv_mem, *],
+  end,
 }
 
 /-- The preimage of a subgroup under a group homomorphism, as a subgroup. -/
 def comap (f : G →** H) (K : subgroup H) : subgroup G :=
 { carrier := {g : G | f g ∈ K },
-  one_mem' := begin sorry end,
-  mul_mem' := begin sorry end,
-  inv_mem' := begin sorry end,
+  one_mem' := begin simp [map_one, K.one_mem], end,
+  mul_mem' :=
+  begin
+    intros a b ha hb,
+    simp [map_mul, K.mul_mem, *] at *,
+  end,
+  inv_mem' :=
+  begin
+    intros x hx,
+    simp [map_inv, K.inv_mem, *] at *,
+  end,
 }
 
 /-- Pushing a subgroup along one homomorphism and then another is equal to
@@ -138,7 +182,29 @@ def comap (f : G →** H) (K : subgroup H) : subgroup G :=
 lemma map_comp (φ : G →** H) (ψ : H →** K) (L : subgroup G) :
   (φ.comp ψ).map L = ψ.map (φ.map L) :=
 begin
-  sorry
+  ext,
+  split,
+  {
+    intro hx,
+    cases hx with x' hx,
+    simp [map, comp, *] at *,
+    use x',
+    split,
+    { exact hx.1 },
+    { exact hx.2 },
+  },
+  {
+    intro hx,
+    cases hx with x' hx,
+    cases hx.1 with x'' hx',
+    use x'',
+    split,
+    { exact hx'.1 },
+    dsimp [comp],
+    have hx := hx.2,
+    rw ←hx'.2 at hx,
+    exact hx,
+  },
 end
 
 /-- Pulling a subgroup back along one homomorphism and then another, is equal
@@ -146,7 +212,16 @@ to pulling it back along the composite of the homomorphisms. -/
 lemma comap_comp (φ : G →** H) (ψ : H →** K) (L : subgroup K) :
   (φ.comp ψ).comap L = φ.comap (ψ.comap L) :=
 begin
-  sorry
+  ext,
+  split,
+  {
+    intro hx,
+    exact hx,
+  },
+  {
+    intro hx,
+    exact hx,
+  }
 end
 
 end my_group_hom
